InferenceInLean/Inference.lean
@@ -30,6 +30,8 @@ instance : Membership (Inference sig X) (InferenceSystem sig X) :=
 
 variable {sig : Signature} {X : Variables} {univ : Universes}
 
+/-- This formalization of proofs is one of several possible translations for the definition in the
+lecture notes, and is the one that ended up being the most ergonomic one to use for us. -/
 structure Proof (Γ : InferenceSystem sig X) where
   assumptions : Set (Clause sig X)
   conclusion : Clause sig X
@@ -43,19 +45,26 @@ structure Proof (Γ : InferenceSystem sig X) where
     ∃ inference ∈ Γ, clauses[i] = inference.conclusion ∧ inference.condition ∧
       ∀ Clause ∈ inference.premises, ∃ (j : ℕ) (hjindex : j < i), Clause = clauses[j]
 
+/-- Syntactic entailment N ⊢ F in Γ. -/
 @[simp]
 def Provability (Γ : InferenceSystem sig X) (N : Set (Clause sig X)) (F : Clause sig X) : Prop :=
   ∃ proof : Proof Γ, proof.assumptions = N ∧ proof.conclusion = F
 
+/-- This is the soundness definition from the lecture notes, which is based on inferences. -/
 @[simp]
 def Soundness [inst : DecidableEq X] (Γ : InferenceSystem sig X) : Prop :=
   ∀ inference ∈ Γ, inference.condition →
     @ClauseSetEntails _ _ univ _ inference.premises inference.conclusion
 
+/-- This is the more general definition for soundness: An inference system Γ is sound if
+N ⊢ F → N ⊨ F. -/
 @[simp]
 def GeneralSoundness [inst : DecidableEq X] (Γ : InferenceSystem sig X) : Prop :=
   ∀ (N : Set (Clause _ _)) (F : Clause _ _), Provability Γ N F → @ClauseSetEntails _ _ univ _ N F
 
+/-- Proof that the more general definition of soundness follows from the inference-based one in
+the lecture notes. This means that we can show the soundness of an inference system Γ just by
+showing that all of its inferences are sound. -/
 theorem generalSoundness_of_soundness [inst : DecidableEq X]
     (Γ : InferenceSystem sig X) : @Soundness _ _ univ _ Γ → @GeneralSoundness _ _ univ _ Γ := by
   intro hsound N F hproof A β hgstrue
